proof/refine/AARCH64/InvariantUpdates_H.thy
@@ -13,6 +13,14 @@ arch_requalify_facts
   cte_wp_atE'
   cte_wp_at_cteI'
   tcb_at_cte_at'
+  typ_at_lift_valid_cap'
+  valid_arch_tcb_lift'
+
+(* arch-specific typ_at_lifts in Arch *)
+lemmas gen_typ_at_lifts =
+         typ_at_lift_tcb' typ_at_lift_ep' typ_at_lift_ntfn' typ_at_lift_cte' typ_at_lift_cte_at'
+         typ_at_lift_valid_untyped' typ_at_lift_valid_cap' valid_bound_tcb_lift
+         valid_arch_tcb_lift'
 
 (* these depend on interpretations in ArchInvLemmas_H *)
 context pspace_update_eq'
